w64x4/proof/Fp_w64x4_extract_ct.ec
@@ -1,378 +1,104 @@
 require import AllCore IntDiv CoreMap List Distr.
 require import JModel.
 
-require import Array4 Array8 Array32.
-require import WArray32 WArray64.
+require import Array4.
+require import WArray32.
 
 
 
 module M = {
   var leakages : leakages_t
   
-  proc bn2_unpack (a:W64.t Array8.t) : W64.t Array4.t * W64.t Array4.t = {
-    var aux: int;
-    var aux_0: W64.t;
-    
-    var hi:W64.t Array4.t;
-    var lo:W64.t Array4.t;
-    var i:int;
-    hi <- witness;
-    lo <- witness;
-    leakages <- LeakFor(0,4) :: LeakAddr([]) :: leakages;
-    i <- 0;
-    while (i < 4) {
-      leakages <- LeakAddr([i]) :: leakages;
-      aux_0 <- a.[i];
-      leakages <- LeakAddr([i]) :: leakages;
-      lo.[i] <- aux_0;
-      leakages <- LeakAddr([(4 + i)]) :: leakages;
-      aux_0 <- a.[(4 + i)];
-      leakages <- LeakAddr([i]) :: leakages;
-      hi.[i] <- aux_0;
-      i <- i + 1;
-    }
-    return (hi, lo);
-  }
-  
-  proc bn_eq (a:W64.t Array4.t, b:W64.t Array4.t) : W64.t = {
-    var aux_5: bool;
-    var aux_4: bool;
-    var aux_3: bool;
-    var aux_2: bool;
-    var aux_1: bool;
-    var aux_0: int;
+  proc bn_subc (a:W64.t Array4.t, b:W64.t Array4.t) : bool * W64.t Array4.t = {
+    var aux_0: bool;
+    var aux_1: int;
     var aux: W64.t;
     
-    var res_0:W64.t;
-    var are_equal:W64.t;
-    var acc:W64.t;
+    var cf:bool;
+    var x1:W64.t;
+    var x2:W64.t;
     var i:int;
-    var t:W64.t;
-    var zf:bool;
-    var  _0:bool;
-    var  _1:bool;
-    var  _2:bool;
-    var  _3:bool;
-    var  _4:W64.t;
     
+    leakages <- LeakAddr([0]) :: leakages;
+    aux <- a.[0];
+    x1 <- aux;
+    leakages <- LeakAddr([0]) :: leakages;
+    aux <- b.[0];
+    x2 <- aux;
     leakages <- LeakAddr([]) :: leakages;
-    aux <- (W64.of_int 0);
-    res_0 <- aux;
+    (aux_0, aux) <- subc_64 x1 x2 false;
+    cf <- aux_0;
+    x1 <- aux;
     leakages <- LeakAddr([]) :: leakages;
-    aux <- (W64.of_int 1);
-    are_equal <- aux;
-    leakages <- LeakAddr([]) :: leakages;
-    aux <- (W64.of_int 0);
-    acc <- aux;
-    leakages <- LeakFor(0,4) :: LeakAddr([]) :: leakages;
-    i <- 0;
+    aux <- x1;
+    leakages <- LeakAddr([0]) :: leakages;
+    a.[0] <- aux;
+    leakages <- LeakFor(1,4) :: LeakAddr([]) :: leakages;
+    i <- 1;
     while (i < 4) {
       leakages <- LeakAddr([i]) :: leakages;
       aux <- a.[i];
-      t <- aux;
+      x1 <- aux;
       leakages <- LeakAddr([i]) :: leakages;
-      aux <- (t `^` b.[i]);
-      t <- aux;
+      aux <- b.[i];
+      x2 <- aux;
       leakages <- LeakAddr([]) :: leakages;
-      aux <- (acc `|` t);
-      acc <- aux;
-      i <- i + 1;
-    }
-    leakages <- LeakAddr([]) :: leakages;
-    (aux_5, aux_4, aux_3, aux_2, aux_1, aux) <- AND_64 acc acc;
-     _0 <- aux_5;
-     _1 <- aux_4;
-     _2 <- aux_3;
-     _3 <- aux_2;
-    zf <- aux_1;
-     _4 <- aux;
-    leakages <- LeakAddr([]) :: leakages;
-    aux <- (zf ? are_equal : res_0);
-    res_0 <- aux;
-    return (res_0);
-  }
-  
-  proc bn_test0 (a:W64.t Array4.t) : W64.t = {
-    var aux_5: bool;
-    var aux_4: bool;
-    var aux_3: bool;
-    var aux_2: bool;
-    var aux_1: bool;
-    var aux_0: int;
-    var aux: W64.t;
-    
-    var res_0:W64.t;
-    var is_zero:W64.t;
-    var acc:W64.t;
-    var i:int;
-    var zf:bool;
-    var  _0:bool;
-    var  _1:bool;
-    var  _2:bool;
-    var  _3:bool;
-    var  _4:W64.t;
-    
-    leakages <- LeakAddr([]) :: leakages;
-    aux <- (W64.of_int 0);
-    res_0 <- aux;
-    leakages <- LeakAddr([]) :: leakages;
-    aux <- (W64.of_int 1);
-    is_zero <- aux;
-    leakages <- LeakAddr([0]) :: leakages;
-    aux <- a.[0];
-    acc <- aux;
-    leakages <- LeakFor(1,4) :: LeakAddr([]) :: leakages;
-    i <- 1;
-    while (i < 4) {
+      (aux_0, aux) <- subc_64 x1 x2 cf;
+      cf <- aux_0;
+      x1 <- aux;
+      leakages <- LeakAddr([]) :: leakages;
+      aux <- x1;
       leakages <- LeakAddr([i]) :: leakages;
-      aux <- (acc `|` a.[i]);
-      acc <- aux;
-      i <- i + 1;
-    }
-    leakages <- LeakAddr([]) :: leakages;
-    (aux_5, aux_4, aux_3, aux_2, aux_1, aux) <- AND_64 acc acc;
-     _0 <- aux_5;
-     _1 <- aux_4;
-     _2 <- aux_3;
-     _3 <- aux_2;
-    zf <- aux_1;
-     _4 <- aux;
-    leakages <- LeakAddr([]) :: leakages;
-    aux <- (zf ? is_zero : res_0);
-    res_0 <- aux;
-    return (res_0);
-  }
-  
-  proc bn_add1 (a:W64.t Array4.t, b:W64.t) : bool * W64.t Array4.t = {
-    var aux: bool;
-    var aux_1: int;
-    var aux_0: W64.t;
-    
-    var cf:bool;
-    var i:int;
-    
-    leakages <- LeakAddr([0]) :: leakages;
-    (aux, aux_0) <- addc_64 a.[0] b false;
-    cf <- aux;
-    leakages <- LeakAddr([0]) :: leakages;
-    a.[0] <- aux_0;
-    leakages <- LeakFor(1,4) :: LeakAddr([]) :: leakages;
-    i <- 1;
-    while (i < 4) {
-      leakages <- LeakAddr([i]) :: leakages;
-      (aux, aux_0) <- addc_64 a.[i] (W64.of_int 0) cf;
-      cf <- aux;
-      leakages <- LeakAddr([i]) :: leakages;
-      a.[i] <- aux_0;
+      a.[i] <- aux;
       i <- i + 1;
     }
     return (cf, a);
   }
   
   proc bn_addc (a:W64.t Array4.t, b:W64.t Array4.t) : bool * W64.t Array4.t = {
-    var aux: bool;
-    var aux_1: int;
-    var aux_0: W64.t;
-    
-    var cf:bool;
-    var i:int;
-    
-    leakages <- LeakAddr([0; 0]) :: leakages;
-    (aux, aux_0) <- addc_64 a.[0] b.[0] false;
-    cf <- aux;
-    leakages <- LeakAddr([0]) :: leakages;
-    a.[0] <- aux_0;
-    leakages <- LeakFor(1,4) :: LeakAddr([]) :: leakages;
-    i <- 1;
-    while (i < 4) {
-      leakages <- LeakAddr([i; i]) :: leakages;
-      (aux, aux_0) <- addc_64 a.[i] b.[i] cf;
-      cf <- aux;
-      leakages <- LeakAddr([i]) :: leakages;
-      a.[i] <- aux_0;
-      i <- i + 1;
-    }
-    return (cf, a);
-  }
-  
-  proc bn_subc (a:W64.t Array4.t, b:W64.t Array4.t) : bool * W64.t Array4.t = {
-    var aux: bool;
-    var aux_1: int;
-    var aux_0: W64.t;
-    
-    var cf:bool;
-    var i:int;
-    
-    leakages <- LeakAddr([0; 0]) :: leakages;
-    (aux, aux_0) <- subc_64 a.[0] b.[0] false;
-    cf <- aux;
-    leakages <- LeakAddr([0]) :: leakages;
-    a.[0] <- aux_0;
-    leakages <- LeakFor(1,4) :: LeakAddr([]) :: leakages;
-    i <- 1;
-    while (i < 4) {
-      leakages <- LeakAddr([i; i]) :: leakages;
-      (aux, aux_0) <- subc_64 a.[i] b.[i] cf;
-      cf <- aux;
-      leakages <- LeakAddr([i]) :: leakages;
-      a.[i] <- aux_0;
-      i <- i + 1;
-    }
-    return (cf, a);
-  }
-  
-  proc mul1 (a:W64.t, b:W64.t Array4.t) : W64.t * bool * bool *
-                                          W64.t Array8.t = {
-    var aux_3: bool;
-    var aux_2: bool;
-    var aux_1: bool;
     var aux_0: bool;
-    var aux: bool;
-    var aux_6: int;
-    var aux_5: W64.t;
-    var aux_4: W64.t;
-    
-    var _zero:W64.t;
-    var of_0:bool;
-    var cf:bool;
-    var r:W64.t Array8.t;
-    var i:int;
-    var lo:W64.t;
-    var  _0:bool;
-    var  _1:bool;
-    var  _2:bool;
-    r <- witness;
-    leakages <- LeakAddr([]) :: leakages;
-    (aux_3, aux_2, aux_1, aux_0, aux, aux_5) <- set0_64 ;
-    of_0 <- aux_3;
-    cf <- aux_2;
-     _0 <- aux_1;
-     _1 <- aux_0;
-     _2 <- aux;
-    _zero <- aux_5;
-    leakages <- LeakAddr([0]) :: leakages;
-    (aux_5, aux_4) <- MULX_64 a b.[0];
-    leakages <- LeakAddr([1]) :: leakages;
-    r.[1] <- aux_5;
-    leakages <- LeakAddr([0]) :: leakages;
-    r.[0] <- aux_4;
-    leakages <- LeakFor(1,4) :: LeakAddr([]) :: leakages;
-    i <- 1;
-    while (i < 4) {
-      leakages <- LeakAddr([i]) :: leakages;
-      (aux_5, aux_4) <- MULX_64 a b.[i];
-      leakages <- LeakAddr([(i + 1)]) :: leakages;
-      r.[(i + 1)] <- aux_5;
-      lo <- aux_4;
-      leakages <- LeakAddr([i]) :: leakages;
-      (aux_3, aux_5) <- ADCX_64 r.[i] lo cf;
-      cf <- aux_3;
-      leakages <- LeakAddr([i]) :: leakages;
-      r.[i] <- aux_5;
-      i <- i + 1;
-    }
-    leakages <- LeakAddr([4]) :: leakages;
-    (aux_3, aux_5) <- ADCX_64 r.[4] _zero cf;
-    cf <- aux_3;
-    leakages <- LeakAddr([4]) :: leakages;
-    r.[4] <- aux_5;
-    return (_zero, of_0, cf, r);
-  }
-  
-  proc mul1acc (k:int, a:W64.t, b:W64.t Array4.t, r:W64.t Array8.t,
-                _zero:W64.t, of_0:bool, cf:bool) : W64.t * bool * bool *
-                                                   W64.t Array8.t = {
-    var aux_2: bool;
-    var aux: int;
-    var aux_1: W64.t;
-    var aux_0: W64.t;
-    
-    var i:int;
-    var hi:W64.t;
-    var lo:W64.t;
-    
-    leakages <- LeakFor(0,(4 - 1)) :: LeakAddr([]) :: leakages;
-    aux <- (4 - 1);
-    i <- 0;
-    while (i < aux) {
-      leakages <- LeakAddr([i]) :: leakages;
-      (aux_1, aux_0) <- MULX_64 a b.[i];
-      hi <- aux_1;
-      lo <- aux_0;
-      leakages <- LeakAddr([(k + i)]) :: leakages;
-      (aux_2, aux_1) <- ADOX_64 r.[(k + i)] lo of_0;
-      of_0 <- aux_2;
-      leakages <- LeakAddr([(k + i)]) :: leakages;
-      r.[(k + i)] <- aux_1;
-      leakages <- LeakAddr([((k + i) + 1)]) :: leakages;
-      (aux_2, aux_1) <- ADCX_64 r.[((k + i) + 1)] hi cf;
-      cf <- aux_2;
-      leakages <- LeakAddr([((k + i) + 1)]) :: leakages;
-      r.[((k + i) + 1)] <- aux_1;
-      i <- i + 1;
-    }
-    leakages <- LeakAddr([(4 - 1)]) :: leakages;
-    (aux_1, aux_0) <- MULX_64 a b.[(4 - 1)];
-    leakages <- LeakAddr([(4 + k)]) :: leakages;
-    r.[(4 + k)] <- aux_1;
-    lo <- aux_0;
-    leakages <- LeakAddr([((4 + k) - 1)]) :: leakages;
-    (aux_2, aux_1) <- ADOX_64 r.[((4 + k) - 1)] lo of_0;
-    of_0 <- aux_2;
-    leakages <- LeakAddr([((4 + k) - 1)]) :: leakages;
-    r.[((4 + k) - 1)] <- aux_1;
-    leakages <- LeakAddr([(4 + k)]) :: leakages;
-    (aux_2, aux_1) <- ADCX_64 r.[(4 + k)] _zero cf;
-    cf <- aux_2;
-    leakages <- LeakAddr([(4 + k)]) :: leakages;
-    r.[(4 + k)] <- aux_1;
-    leakages <- LeakAddr([(4 + k)]) :: leakages;
-    (aux_2, aux_1) <- ADOX_64 r.[(4 + k)] _zero of_0;
-    of_0 <- aux_2;
-    leakages <- LeakAddr([(4 + k)]) :: leakages;
-    r.[(4 + k)] <- aux_1;
-    return (_zero, of_0, cf, r);
-  }
-  
-  proc bn_muln (a:W64.t Array4.t, b:W64.t Array4.t) : W64.t * bool * bool *
-                                                      W64.t Array8.t = {
-    var aux_1: bool;
-    var aux_0: bool;
-    var aux_3: int;
+    var aux_1: int;
     var aux: W64.t;
-    var aux_2: W64.t Array8.t;
     
-    var _zero:W64.t;
-    var of_0:bool;
     var cf:bool;
-    var r:W64.t Array8.t;
-    var ai:W64.t;
+    var x1:W64.t;
+    var x2:W64.t;
     var i:int;
-    r <- witness;
+    
     leakages <- LeakAddr([0]) :: leakages;
     aux <- a.[0];
-    ai <- aux;
+    x1 <- aux;
+    leakages <- LeakAddr([0]) :: leakages;
+    aux <- b.[0];
+    x2 <- aux;
     leakages <- LeakAddr([]) :: leakages;
-    (aux, aux_1, aux_0, aux_2) <@ mul1 (ai, b);
-    _zero <- aux;
-    of_0 <- aux_1;
+    (aux_0, aux) <- addc_64 x1 x2 false;
     cf <- aux_0;
-    r <- aux_2;
+    x1 <- aux;
+    leakages <- LeakAddr([]) :: leakages;
+    aux <- x1;
+    leakages <- LeakAddr([0]) :: leakages;
+    a.[0] <- aux;
     leakages <- LeakFor(1,4) :: LeakAddr([]) :: leakages;
     i <- 1;
     while (i < 4) {
       leakages <- LeakAddr([i]) :: leakages;
       aux <- a.[i];
-      ai <- aux;
+      x1 <- aux;
+      leakages <- LeakAddr([i]) :: leakages;
+      aux <- b.[i];
+      x2 <- aux;
       leakages <- LeakAddr([]) :: leakages;
-      (aux, aux_1, aux_0, aux_2) <@ mul1acc (i, ai, b, r, _zero, of_0, cf);
-      _zero <- aux;
-      of_0 <- aux_1;
+      (aux_0, aux) <- addc_64 x1 x2 cf;
       cf <- aux_0;
-      r <- aux_2;
+      x1 <- aux;
+      leakages <- LeakAddr([]) :: leakages;
+      aux <- x1;
+      leakages <- LeakAddr([i]) :: leakages;
+      a.[i] <- aux;
       i <- i + 1;
     }
-    return (_zero, of_0, cf, r);
+    return (cf, a);
   }
   
   proc ith_bit64 (k:W64.t, ctr:W64.t) : W64.t = {
@@ -403,15 +129,23 @@ module M = {
     var aux: W64.t;
     
     var bit:W64.t;
+    var ctr2:W64.t;
+    var ctr3:W64.t;
     var c1:W64.t;
     var c2:W64.t;
     var r:W64.t;
     
     leakages <- LeakAddr([]) :: leakages;
-    aux <- (ctr `>>` (W8.of_int 6));
+    aux <- ctr;
+    ctr2 <- aux;
+    leakages <- LeakAddr([]) :: leakages;
+    aux <- ctr;
+    ctr3 <- aux;
+    leakages <- LeakAddr([]) :: leakages;
+    aux <- (ctr2 `>>` (W8.of_int 6));
     c1 <- aux;
     leakages <- LeakAddr([]) :: leakages;
-    aux <- (ctr - (c1 * (W64.of_int 64)));
+    aux <- (ctr3 `&` (W64.of_int 63));
     c2 <- aux;
     leakages <- LeakAddr([(W64.to_uint c1)]) :: leakages;
     aux <- kk.[(W64.to_uint c1)];
@@ -466,492 +200,135 @@ module M = {
     return (x, y);
   }
   
-  proc maskOnCarry (mask:int, r:W64.t, _cf:bool) : W64.t = {
-    var aux: bool;
-    var aux_0: W64.t;
-    
-    
-    
-    leakages <- LeakAddr([]) :: leakages;
-    (aux, aux_0) <- subc_64 r r _cf;
-    _cf <- aux;
-    r <- aux_0;
-    leakages <- LeakAddr([]) :: leakages;
-    aux_0 <- (r `&` (W64.of_int mask));
-    r <- aux_0;
-    return (r);
-  }
-  
-  proc x2r (x0:W64.t, x1:W64.t, x2:W64.t, x3:W64.t) : W64.t Array4.t = {
+  proc cminusP (p:W64.t Array4.t, x:W64.t Array4.t) : W64.t Array4.t = {
+    var aux_0: bool;
     var aux: W64.t;
+    var aux_1: W64.t Array4.t;
     
-    var r:W64.t Array4.t;
-    r <- witness;
-    leakages <- LeakAddr([]) :: leakages;
-    aux <- x0;
-    leakages <- LeakAddr([0]) :: leakages;
-    r.[0] <- aux;
-    leakages <- LeakAddr([]) :: leakages;
-    aux <- x1;
-    leakages <- LeakAddr([1]) :: leakages;
-    r.[1] <- aux;
-    leakages <- LeakAddr([]) :: leakages;
-    aux <- x2;
-    leakages <- LeakAddr([2]) :: leakages;
-    r.[2] <- aux;
-    leakages <- LeakAddr([]) :: leakages;
-    aux <- x3;
-    leakages <- LeakAddr([3]) :: leakages;
-    r.[3] <- aux;
-    return (r);
-  }
-  
-  proc r2x (x:W64.t Array4.t) : W64.t * W64.t * W64.t * W64.t = {
-    var aux: W64.t;
-    
-    var r0:W64.t;
+    var t:W64.t Array4.t;
+    var z:W64.t Array4.t;
+    var cf:bool;
     var r1:W64.t;
     var r2:W64.t;
-    var r3:W64.t;
-    
+    t <- witness;
+    z <- witness;
     leakages <- LeakAddr([0]) :: leakages;
     aux <- x.[0];
-    r0 <- aux;
+    leakages <- LeakAddr([0]) :: leakages;
+    z.[0] <- aux;
     leakages <- LeakAddr([1]) :: leakages;
     aux <- x.[1];
+    leakages <- LeakAddr([1]) :: leakages;
+    z.[1] <- aux;
+    leakages <- LeakAddr([2]) :: leakages;
+    aux <- x.[2];
+    leakages <- LeakAddr([2]) :: leakages;
+    z.[2] <- aux;
+    leakages <- LeakAddr([3]) :: leakages;
+    aux <- x.[3];
+    leakages <- LeakAddr([3]) :: leakages;
+    z.[3] <- aux;
+    leakages <- LeakAddr([]) :: leakages;
+    (aux_0, aux_1) <@ bn_subc (z, p);
+    cf <- aux_0;
+    t <- aux_1;
+    leakages <- LeakAddr([0]) :: leakages;
+    aux <- t.[0];
+    r1 <- aux;
+    leakages <- LeakAddr([0]) :: leakages;
+    aux <- x.[0];
+    r2 <- aux;
+    leakages <- LeakAddr([]) :: leakages;
+    aux <- (cf ? r2 : r1);
+    r1 <- aux;
+    leakages <- LeakAddr([]) :: leakages;
+    aux <- r1;
+    leakages <- LeakAddr([0]) :: leakages;
+    t.[0] <- aux;
+    leakages <- LeakAddr([1]) :: leakages;
+    aux <- t.[1];
+    r1 <- aux;
+    leakages <- LeakAddr([1]) :: leakages;
+    aux <- x.[1];
+    r2 <- aux;
+    leakages <- LeakAddr([]) :: leakages;
+    aux <- (cf ? r2 : r1);
+    r1 <- aux;
+    leakages <- LeakAddr([]) :: leakages;
+    aux <- r1;
+    leakages <- LeakAddr([1]) :: leakages;
+    t.[1] <- aux;
+    leakages <- LeakAddr([2]) :: leakages;
+    aux <- t.[2];
     r1 <- aux;
     leakages <- LeakAddr([2]) :: leakages;
     aux <- x.[2];
     r2 <- aux;
+    leakages <- LeakAddr([]) :: leakages;
+    aux <- (cf ? r2 : r1);
+    r1 <- aux;
+    leakages <- LeakAddr([]) :: leakages;
+    aux <- r1;
+    leakages <- LeakAddr([2]) :: leakages;
+    t.[2] <- aux;
+    leakages <- LeakAddr([3]) :: leakages;
+    aux <- t.[3];
+    r1 <- aux;
     leakages <- LeakAddr([3]) :: leakages;
     aux <- x.[3];
-    r3 <- aux;
-    return (r0, r1, r2, r3);
+    r2 <- aux;
+    leakages <- LeakAddr([]) :: leakages;
+    aux <- (cf ? r2 : r1);
+    r1 <- aux;
+    leakages <- LeakAddr([]) :: leakages;
+    aux <- r1;
+    leakages <- LeakAddr([3]) :: leakages;
+    t.[3] <- aux;
+    return (t);
   }
   
-  proc cminusP (x:W64.t Array4.t) : W64.t Array4.t = {
-    var aux_2: bool;
+  proc addm (p:W64.t Array4.t, a:W64.t Array4.t, b:W64.t Array4.t) : 
+  W64.t Array4.t = {
+    var aux: bool;
     var aux_1: W64.t;
-    var aux: W8.t Array32.t;
     var aux_0: W64.t Array4.t;
     
-    var t:W64.t Array4.t;
-    var twop63:W64.t;
-    var cf:bool;
-    t <- witness;
-    leakages <- LeakAddr([]) :: leakages;
-    aux_0 <-  x;
-    t <- aux_0;
-    leakages <- LeakAddr([]) :: leakages;
-    aux_1 <- (W64.of_int 1);
-    twop63 <- aux_1;
-    leakages <- LeakAddr([]) :: leakages;
-    aux_1 <- (twop63 `<<` (W8.of_int 63));
-    twop63 <- aux_1;
-    leakages <- LeakAddr([0]) :: leakages;
-    (aux_2, aux_1) <- addc_64 t.[0] (W64.of_int 19) false;
-    cf <- aux_2;
-    leakages <- LeakAddr([0]) :: leakages;
-    t.[0] <- aux_1;
-    leakages <- LeakAddr([1]) :: leakages;
-    (aux_2, aux_1) <- addc_64 t.[1] (W64.of_int 0) cf;
-    cf <- aux_2;
-    leakages <- LeakAddr([1]) :: leakages;
-    t.[1] <- aux_1;
-    leakages <- LeakAddr([2]) :: leakages;
-    (aux_2, aux_1) <- addc_64 t.[2] (W64.of_int 0) cf;
-    cf <- aux_2;
-    leakages <- LeakAddr([2]) :: leakages;
-    t.[2] <- aux_1;
-    leakages <- LeakAddr([3]) :: leakages;
-    (aux_2, aux_1) <- addc_64 t.[3] twop63 cf;
-    cf <- aux_2;
-    leakages <- LeakAddr([3]) :: leakages;
-    t.[3] <- aux_1;
-    leakages <- LeakAddr([0; 0]) :: leakages;
-    aux_1 <- (cf ? t.[0] : x.[0]);
-    leakages <- LeakAddr([0]) :: leakages;
-    x.[0] <- aux_1;
-    leakages <- LeakAddr([1; 1]) :: leakages;
-    aux_1 <- (cf ? t.[1] : x.[1]);
-    leakages <- LeakAddr([1]) :: leakages;
-    x.[1] <- aux_1;
-    leakages <- LeakAddr([2; 2]) :: leakages;
-    aux_1 <- (cf ? t.[2] : x.[2]);
-    leakages <- LeakAddr([2]) :: leakages;
-    x.[2] <- aux_1;
-    leakages <- LeakAddr([3; 3]) :: leakages;
-    aux_1 <- (cf ? t.[3] : x.[3]);
-    leakages <- LeakAddr([3]) :: leakages;
-    x.[3] <- aux_1;
-    return (x);
-  }
-  
-  proc caddP (cf:bool, x:W64.t Array4.t) : W64.t Array4.t = {
-    var aux_0: bool;
-    var aux: W64.t;
-    var aux_1: W64.t Array4.t;
-    
-    var p:W64.t Array4.t;
-    var _zero:W64.t;
+    var f:W64.t Array4.t;
+    var z:W64.t Array4.t;
     var  _0:bool;
-    p <- witness;
+    f <- witness;
+    z <- witness;
     leakages <- LeakAddr([]) :: leakages;
-    aux <- (W64.of_int 18446744073709551597);
+    (aux, aux_0) <@ bn_addc (a, b);
+     _0 <- aux;
+    f <- aux_0;
     leakages <- LeakAddr([0]) :: leakages;
-    p.[0] <- aux;
-    leakages <- LeakAddr([]) :: leakages;
-    aux <- (W64.of_int 18446744073709551615);
-    leakages <- LeakAddr([1]) :: leakages;
-    p.[1] <- aux;
-    leakages <- LeakAddr([]) :: leakages;
-    aux <- (W64.of_int 18446744073709551615);
-    leakages <- LeakAddr([2]) :: leakages;
-    p.[2] <- aux;
-    leakages <- LeakAddr([]) :: leakages;
-    aux <- (W64.of_int 9223372036854775807);
-    leakages <- LeakAddr([3]) :: leakages;
-    p.[3] <- aux;
-    leakages <- LeakAddr([]) :: leakages;
-    aux <- (W64.of_int 0);
-    _zero <- aux;
+    aux_1 <- f.[0];
     leakages <- LeakAddr([0]) :: leakages;
-    aux <- ((! cf) ? _zero : p.[0]);
-    leakages <- LeakAddr([0]) :: leakages;
-    p.[0] <- aux;
+    z.[0] <- aux_1;
     leakages <- LeakAddr([1]) :: leakages;
-    aux <- ((! cf) ? _zero : p.[1]);
+    aux_1 <- f.[1];
     leakages <- LeakAddr([1]) :: leakages;
-    p.[1] <- aux;
+    z.[1] <- aux_1;
     leakages <- LeakAddr([2]) :: leakages;
-    aux <- ((! cf) ? _zero : p.[2]);
+    aux_1 <- f.[2];
     leakages <- LeakAddr([2]) :: leakages;
-    p.[2] <- aux;
+    z.[2] <- aux_1;
     leakages <- LeakAddr([3]) :: leakages;
-    aux <- ((! cf) ? _zero : p.[3]);
+    aux_1 <- f.[3];
     leakages <- LeakAddr([3]) :: leakages;
-    p.[3] <- aux;
+    z.[3] <- aux_1;
     leakages <- LeakAddr([]) :: leakages;
-    (aux_0, aux_1) <@ bn_addc (x, p);
-     _0 <- aux_0;
-    x <- aux_1;
-    return (x);
+    aux_0 <@ cminusP (p, z);
+    f <- aux_0;
+    return (f);
   }
   
-  proc redp25519 (_of:bool, _cf:bool, a:W64.t Array8.t) : W64.t Array4.t = {
-    var aux_7: bool;
-    var aux_6: bool;
-    var aux_5: bool;
-    var aux_3: bool;
-    var aux_2: bool;
+  proc mulm (m:W64.t Array4.t, x:W64.t Array4.t, n:W64.t Array4.t) : 
+  W64.t Array4.t = {
     var aux: W64.t;
     var aux_1: W64.t Array4.t;
     var aux_0: W64.t Array4.t;
-    var aux_4: W64.t Array8.t;
-    
-    var al:W64.t Array4.t;
-    var tmp:W64.t;
-    var _zero:W64.t;
-    var ah:W64.t Array4.t;
-    var  _0:W64.t Array4.t;
-    var  _1:bool;
-    var  _2:bool;
-    var  _3:bool;
-    var  _4:bool;
-    var  _5:bool;
-    var  _6:W64.t Array4.t;
-     _0 <- witness;
-     _6 <- witness;
-    ah <- witness;
-    al <- witness;
-    leakages <- LeakAddr([]) :: leakages;
-    aux <- (W64.of_int 38);
-    tmp <- aux;
-    leakages <- LeakAddr([]) :: leakages;
-    aux <- (W64.of_int 0);
-    _zero <- aux;
-    leakages <- LeakAddr([]) :: leakages;
-    (aux_1, aux_0) <@ bn2_unpack (a);
-    ah <- aux_1;
-     _0 <- aux_0;
-    leakages <- LeakAddr([]) :: leakages;
-    (aux, aux_7, aux_6, aux_4) <@ mul1acc (0, tmp, ah, a, _zero, _of, _cf);
-    _zero <- aux;
-    _of <- aux_7;
-    _cf <- aux_6;
-    a <- aux_4;
-    leakages <- LeakAddr([4]) :: leakages;
-    (aux_7, aux_6, aux_5, aux_3, aux_2, aux) <- IMULri_64 a.[4]
-    (W64.of_int 38);
-     _1 <- aux_7;
-     _2 <- aux_6;
-     _3 <- aux_5;
-     _4 <- aux_3;
-     _5 <- aux_2;
-    tmp <- aux;
-    leakages <- LeakAddr([]) :: leakages;
-    (aux_1, aux_0) <@ bn2_unpack (a);
-     _6 <- aux_1;
-    al <- aux_0;
-    leakages <- LeakAddr([]) :: leakages;
-    (aux_7, aux_1) <@ bn_add1 (al, tmp);
-    _cf <- aux_7;
-    al <- aux_1;
-    leakages <- LeakAddr([]) :: leakages;
-    aux <@ maskOnCarry (38, tmp, _cf);
-    tmp <- aux;
-    leakages <- LeakAddr([0]) :: leakages;
-    aux <- (al.[0] + tmp);
-    leakages <- LeakAddr([0]) :: leakages;
-    al.[0] <- aux;
-    return (al);
-  }
-  
-  proc freeze (x:W64.t Array4.t) : W64.t Array4.t = {
-    var aux: W64.t Array4.t;
-    
-    
-    
-    leakages <- LeakAddr([]) :: leakages;
-    aux <@ cminusP (x);
-    x <- aux;
-    leakages <- LeakAddr([]) :: leakages;
-    aux <@ cminusP (x);
-    x <- aux;
-    return (x);
-  }
-  
-  proc _mulm (f:W64.t Array4.t, g0:W64.t, g1:W64.t, g2:W64.t, g3:W64.t) : 
-  W64.t * W64.t * W64.t * W64.t = {
-    var aux_2: bool;
-    var aux_1: bool;
-    var aux_6: W64.t;
-    var aux_5: W64.t;
-    var aux_4: W64.t;
-    var aux_0: W64.t;
-    var aux: W64.t Array4.t;
-    var aux_3: W64.t Array8.t;
-    
-    var g:W64.t Array4.t;
-    var _zero:W64.t;
-    var of_0:bool;
-    var cf:bool;
-    var h:W64.t Array8.t;
-    g <- witness;
-    h <- witness;
-    leakages <- LeakAddr([]) :: leakages;
-    aux <@ x2r (g0, g1, g2, g3);
-    g <- aux;
-    leakages <- LeakAddr([]) :: leakages;
-    (aux_6, aux_2, aux_1, aux_3) <@ bn_muln (f, g);
-    _zero <- aux_6;
-    of_0 <- aux_2;
-    cf <- aux_1;
-    h <- aux_3;
-    leakages <- LeakAddr([]) :: leakages;
-    aux <@ redp25519 (of_0, cf, h);
-    g <- aux;
-    leakages <- LeakAddr([]) :: leakages;
-    aux <@ freeze (g);
-    g <- aux;
-    leakages <- LeakAddr([]) :: leakages;
-    (aux_6, aux_5, aux_4, aux_0) <@ r2x (g);
-    g0 <- aux_6;
-    g1 <- aux_5;
-    g2 <- aux_4;
-    g3 <- aux_0;
-    return (g0, g1, g2, g3);
-  }
-  
-  proc mulm (p:W64.t Array4.t, a:W64.t Array4.t, b:W64.t Array4.t) : 
-  W64.t Array4.t = {
-    var aux_2: W64.t;
-    var aux_1: W64.t;
-    var aux_0: W64.t;
-    var aux: W64.t;
-    var aux_3: W64.t Array4.t;
-    
-    var g0:W64.t;
-    var g1:W64.t;
-    var g2:W64.t;
-    var g3:W64.t;
-    
-    leakages <- LeakAddr([]) :: leakages;
-    (aux_2, aux_1, aux_0, aux) <@ r2x (b);
-    g0 <- aux_2;
-    g1 <- aux_1;
-    g2 <- aux_0;
-    g3 <- aux;
-    leakages <- LeakAddr([]) :: leakages;
-    (aux_2, aux_1, aux_0, aux) <@ _mulm (a, g0, g1, g2, g3);
-    g0 <- aux_2;
-    g1 <- aux_1;
-    g2 <- aux_0;
-    g3 <- aux;
-    leakages <- LeakAddr([]) :: leakages;
-    aux_3 <@ x2r (g0, g1, g2, g3);
-    b <- aux_3;
-    return (b);
-  }
-  
-  proc _addm (f0:W64.t, f1:W64.t, f2:W64.t, f3:W64.t, g0:W64.t, g1:W64.t,
-              g2:W64.t, g3:W64.t) : W64.t * W64.t * W64.t * W64.t = {
-    var aux_0: bool;
-    var aux_4: W64.t;
-    var aux_3: W64.t;
-    var aux_2: W64.t;
-    var aux_1: W64.t;
-    var aux: W64.t Array4.t;
-    
-    var f:W64.t Array4.t;
-    var g:W64.t Array4.t;
-    var  _0:bool;
-    f <- witness;
-    g <- witness;
-    leakages <- LeakAddr([]) :: leakages;
-    aux <@ x2r (f0, f1, f2, f3);
-    f <- aux;
-    leakages <- LeakAddr([]) :: leakages;
-    aux <@ x2r (g0, g1, g2, g3);
-    g <- aux;
-    leakages <- LeakAddr([]) :: leakages;
-    (aux_0, aux) <@ bn_addc (f, g);
-     _0 <- aux_0;
-    f <- aux;
-    leakages <- LeakAddr([]) :: leakages;
-    aux <@ cminusP (f);
-    f <- aux;
-    leakages <- LeakAddr([]) :: leakages;
-    (aux_4, aux_3, aux_2, aux_1) <@ r2x (f);
-    f0 <- aux_4;
-    f1 <- aux_3;
-    f2 <- aux_2;
-    f3 <- aux_1;
-    return (f0, f1, f2, f3);
-  }
-  
-  proc addm (a:W64.t Array4.t, b:W64.t Array4.t) : W64.t Array4.t = {
-    var aux_2: W64.t;
-    var aux_1: W64.t;
-    var aux_0: W64.t;
-    var aux: W64.t;
-    var aux_3: W64.t Array4.t;
-    
-    var f0:W64.t;
-    var f1:W64.t;
-    var f2:W64.t;
-    var f3:W64.t;
-    var g0:W64.t;
-    var g1:W64.t;
-    var g2:W64.t;
-    var g3:W64.t;
-    
-    leakages <- LeakAddr([]) :: leakages;
-    (aux_2, aux_1, aux_0, aux) <@ r2x (a);
-    f0 <- aux_2;
-    f1 <- aux_1;
-    f2 <- aux_0;
-    f3 <- aux;
-    leakages <- LeakAddr([]) :: leakages;
-    (aux_2, aux_1, aux_0, aux) <@ r2x (b);
-    g0 <- aux_2;
-    g1 <- aux_1;
-    g2 <- aux_0;
-    g3 <- aux;
-    leakages <- LeakAddr([]) :: leakages;
-    (aux_2, aux_1, aux_0, aux) <@ _addm (f0, f1, f2, f3, g0, g1, g2, g3);
-    f0 <- aux_2;
-    f1 <- aux_1;
-    f2 <- aux_0;
-    f3 <- aux;
-    leakages <- LeakAddr([]) :: leakages;
-    aux_3 <@ x2r (f0, f1, f2, f3);
-    a <- aux_3;
-    return (a);
-  }
-  
-  proc _subm (f0:W64.t, f1:W64.t, f2:W64.t, f3:W64.t, g0:W64.t, g1:W64.t,
-              g2:W64.t, g3:W64.t) : W64.t * W64.t * W64.t * W64.t = {
-    var aux_0: bool;
-    var aux_4: W64.t;
-    var aux_3: W64.t;
-    var aux_2: W64.t;
-    var aux_1: W64.t;
-    var aux: W64.t Array4.t;
-    
-    var f:W64.t Array4.t;
-    var g:W64.t Array4.t;
-    var cf:bool;
-    f <- witness;
-    g <- witness;
-    leakages <- LeakAddr([]) :: leakages;
-    aux <@ x2r (f0, f1, f2, f3);
-    f <- aux;
-    leakages <- LeakAddr([]) :: leakages;
-    aux <@ x2r (g0, g1, g2, g3);
-    g <- aux;
-    leakages <- LeakAddr([]) :: leakages;
-    (aux_0, aux) <@ bn_subc (f, g);
-    cf <- aux_0;
-    f <- aux;
-    leakages <- LeakAddr([]) :: leakages;
-    aux <@ caddP (cf, f);
-    f <- aux;
-    leakages <- LeakAddr([]) :: leakages;
-    (aux_4, aux_3, aux_2, aux_1) <@ r2x (f);
-    f0 <- aux_4;
-    f1 <- aux_3;
-    f2 <- aux_2;
-    f3 <- aux_1;
-    return (f0, f1, f2, f3);
-  }
-  
-  proc subm (a:W64.t Array4.t, b:W64.t Array4.t) : W64.t Array4.t = {
-    var aux_2: W64.t;
-    var aux_1: W64.t;
-    var aux_0: W64.t;
-    var aux: W64.t;
-    var aux_3: W64.t Array4.t;
-    
-    var f0:W64.t;
-    var f1:W64.t;
-    var f2:W64.t;
-    var f3:W64.t;
-    var g0:W64.t;
-    var g1:W64.t;
-    var g2:W64.t;
-    var g3:W64.t;
-    
-    leakages <- LeakAddr([]) :: leakages;
-    (aux_2, aux_1, aux_0, aux) <@ r2x (a);
-    f0 <- aux_2;
-    f1 <- aux_1;
-    f2 <- aux_0;
-    f3 <- aux;
-    leakages <- LeakAddr([]) :: leakages;
-    (aux_2, aux_1, aux_0, aux) <@ r2x (b);
-    g0 <- aux_2;
-    g1 <- aux_1;
-    g2 <- aux_0;
-    g3 <- aux;
-    leakages <- LeakAddr([]) :: leakages;
-    (aux_2, aux_1, aux_0, aux) <@ _subm (f0, f1, f2, f3, g0, g1, g2, g3);
-    f0 <- aux_2;
-    f1 <- aux_1;
-    f2 <- aux_0;
-    f3 <- aux;
-    leakages <- LeakAddr([]) :: leakages;
-    aux_3 <@ x2r (f0, f1, f2, f3);
-    a <- aux_3;
-    return (a);
-  }
-  
-  proc expm (m:W64.t Array4.t, x:W64.t Array4.t, n:W64.t Array4.t) : 
-  W64.t Array4.t = {
-    var aux: W64.t;
-    var aux_0: W8.t Array32.t;
-    var aux_2: W64.t Array4.t;
-    var aux_1: W64.t Array4.t;
     
     var x1:W64.t Array4.t;
     var ctr:W64.t;
@@ -974,7 +351,7 @@ module M = {
     aux <- (W64.of_int ((4 * 64) - 1));
     ctr <- aux;
     leakages <- LeakAddr([]) :: leakages;
-    aux <- (W64.of_int 1);
+    aux <- (W64.of_int 0);
     leakages <- LeakAddr([0]) :: leakages;
     x1.[0] <- aux;
     leakages <- LeakAddr([]) :: leakages;
@@ -990,7 +367,7 @@ module M = {
     leakages <- LeakAddr([3]) :: leakages;
     x1.[3] <- aux;
     leakages <- LeakAddr([]) :: leakages;
-    aux <- (W64.of_int 1);
+    aux <- (W64.of_int 0);
     leakages <- LeakAddr([0]) :: leakages;
     x2.[0] <- aux;
     leakages <- LeakAddr([]) :: leakages;
@@ -1008,23 +385,36 @@ module M = {
     leakages <- LeakAddr([]) :: leakages;
     aux <@ ith_bit (n, ctr);
     d <- aux;
+    leakages <- LeakAddr([0]) :: leakages;
+    aux <- x.[0];
+    leakages <- LeakAddr([0]) :: leakages;
+    x3.[0] <- aux;
+    leakages <- LeakAddr([1]) :: leakages;
+    aux <- x.[1];
+    leakages <- LeakAddr([1]) :: leakages;
+    x3.[1] <- aux;
+    leakages <- LeakAddr([2]) :: leakages;
+    aux <- x.[2];
+    leakages <- LeakAddr([2]) :: leakages;
+    x3.[2] <- aux;
+    leakages <- LeakAddr([3]) :: leakages;
+    aux <- x.[3];
+    leakages <- LeakAddr([3]) :: leakages;
+    x3.[3] <- aux;
     leakages <- LeakAddr([]) :: leakages;
-    aux_2 <-  x;
-    x3 <- aux_2;
-    leakages <- LeakAddr([]) :: leakages;
-    aux_2 <@ mulm (m, x, x);
-    x4 <- aux_2;
+    aux_1 <@ addm (m, x, x);
+    x4 <- aux_1;
     leakages <- LeakAddr([]) :: leakages;
     aux <- d;
     p <- aux;
     leakages <- LeakAddr([]) :: leakages;
-    (aux_2, aux_1) <@ swapr (x1, x3, d);
-    x1 <- aux_2;
-    x3 <- aux_1;
+    (aux_1, aux_0) <@ swapr (x1, x3, d);
+    x1 <- aux_1;
+    x3 <- aux_0;
     leakages <- LeakAddr([]) :: leakages;
-    (aux_2, aux_1) <@ swapr (x2, x4, d);
-    x2 <- aux_2;
-    x4 <- aux_1;
+    (aux_1, aux_0) <@ swapr (x2, x4, d);
+    x2 <- aux_1;
+    x4 <- aux_0;
     
     leakages <- LeakCond(((W64.of_int 0) \ult ctr)) :: LeakAddr([]) :: leakages;
     
@@ -1054,15 +444,15 @@ module M = {
       aux <- (t1 `^` t2);
       par <- aux;
       leakages <- LeakAddr([]) :: leakages;
-      (aux_2, aux_1) <@ swapr (x1, x2, par);
-      x1 <- aux_2;
+      (aux_1, aux_0) <@ swapr (x1, x2, par);
+      x1 <- aux_1;
+      x2 <- aux_0;
+      leakages <- LeakAddr([]) :: leakages;
+      aux_1 <@ addm (m, x1, x2);
+      x1 <- aux_1;
+      leakages <- LeakAddr([]) :: leakages;
+      aux_1 <@ addm (m, x2, x2);
       x2 <- aux_1;
-      leakages <- LeakAddr([]) :: leakages;
-      aux_2 <@ mulm (m, x1, x2);
-      x1 <- aux_2;
-      leakages <- LeakAddr([]) :: leakages;
-      aux_2 <@ mulm (m, x2, x2);
-      x2 <- aux_2;
       leakages <- LeakAddr([]) :: leakages;
       aux <- (q `|` t2);
       q <- aux;
@@ -1070,13 +460,13 @@ module M = {
       aux <- (q `^` p);
       cbit <- aux;
       leakages <- LeakAddr([]) :: leakages;
-      (aux_2, aux_1) <@ swapr (x1, x3, cbit);
-      x1 <- aux_2;
-      x3 <- aux_1;
+      (aux_1, aux_0) <@ swapr (x1, x3, cbit);
+      x1 <- aux_1;
+      x3 <- aux_0;
       leakages <- LeakAddr([]) :: leakages;
-      (aux_2, aux_1) <@ swapr (x2, x4, cbit);
-      x2 <- aux_2;
-      x4 <- aux_1;
+      (aux_1, aux_0) <@ swapr (x2, x4, cbit);
+      x2 <- aux_1;
+      x4 <- aux_0;
     leakages <- LeakCond(((W64.of_int 0) \ult ctr)) :: LeakAddr([]) :: leakages;
     
     }
@@ -1084,59 +474,26 @@ module M = {
     aux <@ ith_bit (n, (W64.of_int 0));
     par <- aux;
     leakages <- LeakAddr([]) :: leakages;
-    (aux_2, aux_1) <@ swapr (x2, x1, par);
-    x1 <- aux_2;
-    x2 <- aux_1;
+    (aux_1, aux_0) <@ swapr (x2, x1, par);
+    x1 <- aux_1;
+    x2 <- aux_0;
     return (x1);
   }
   
   proc toEC () : unit = {
-    var aux_2: bool;
-    var aux_0: W64.t;
-    var aux_1: W64.t Array4.t;
     var aux: W64.t Array4.t;
     
+    var p:W64.t Array4.t;
     var a:W64.t Array4.t;
     var b:W64.t Array4.t;
     var r:W64.t Array4.t;
-    var x:W64.t;
-    var _cf:bool;
-    var  _0:W64.t Array4.t;
-     _0 <- witness;
     a <- witness;
     b <- witness;
+    p <- witness;
     r <- witness;
     leakages <- LeakAddr([]) :: leakages;
-    aux_1 <@ addm (a, b);
-    r <- aux_1;
-    leakages <- LeakAddr([]) :: leakages;
-    aux_1 <@ subm (a, b);
-    r <- aux_1;
-    leakages <- LeakAddr([]) :: leakages;
-    aux_1 <@ mulm (a, a, b);
-    r <- aux_1;
-    leakages <- LeakAddr([]) :: leakages;
-    aux_1 <@ expm (a, a, b);
-    r <- aux_1;
-    leakages <- LeakAddr([]) :: leakages;
-    aux_0 <@ ith_bit (a, x);
-    x <- aux_0;
-    leakages <- LeakAddr([]) :: leakages;
-    (aux_1, aux) <@ swapr (a, a, x);
-     _0 <- aux_1;
-    a <- aux;
-    leakages <- LeakAddr([]) :: leakages;
-    aux_0 <@ bn_eq (a, b);
-    x <- aux_0;
-    leakages <- LeakAddr([]) :: leakages;
-    aux_0 <@ bn_test0 (a);
-    x <- aux_0;
-    leakages <- LeakAddr([]) :: leakages;
-    aux_2 <- false;
-    _cf <- aux_2;
-    leakages <- LeakAddr([]) :: leakages;
-    aux_0 <@ maskOnCarry (7, x, _cf);
-    x <- aux_0;
+    aux <@ mulm (p, a, b);
+    r <- aux;
     return ();
   }
 }.
