w64x4/proof/Fp_w64x4_extract_ct_proof.ec
@@ -2,6 +2,6 @@ require import Fp_w64x4_extract_ct.
 
 
 equiv fp_w64x4_ct :
-  M.expm ~ M.expm :
+  M.mulm ~ M.mulm :
   ={M.leakages, glob M} ==> ={M.leakages}.
 proof. proc; inline *; sim. qed.
